coq/NormalFormProofs.v
@@ -1,0 +1,88 @@
+Require Import Coq.Strings.Ascii.
+Require Import Koika.BitsToLists Koika.Environments Koika.Normalize
+  Koika.TypeInference Koika.UntypedSemantics.
+
+Section NormalForm.
+  Context {pos_t reg_t ext_fn_t rule_name_t: Type}.
+  Context {reg_t_eq_dec: EqDec reg_t}.
+  Context {ext_fn_t_eq_dec: EqDec ext_fn_t}.
+  Context {REnv: Env reg_t}.
+  Context {TR: reg_t -> type}.
+
+  Context (R: reg_t -> type).
+  Context (Sigma: ext_fn_t -> ExternalSignature).
+
+  Definition uact := @uaction pos_t string string reg_t ext_fn_t.
+  Definition schedule := scheduler pos_t rule_name_t.
+  Definition ext_funs_defs :=
+    forall f: ext_fn_t, BitsToLists.val -> BitsToLists.val.
+  Definition UREnv := REnv.(env_t) (fun _ => BitsToLists.val).
+
+  Fixpoint get_vars_in_simpl_uact (e: uact) : list string :=
+    match e with
+    | UBinop ufn a1 a2 =>
+      (get_vars_in_simpl_uact a1)++(get_vars_in_simpl_uact a2)
+    | UUnop ufn a1 => get_vars_in_simpl_uact a1
+    | UVar v => [v]
+    | UIf cond tb fb =>
+      (get_vars_in_simpl_uact cond)
+      ++(get_vars_in_simpl_uact tb)
+      ++(get_vars_in_simpl_uact fb)
+    | _ => [] (* Should never happen *)
+    end.
+
+  (* *)
+  (* R can depend on A *)
+  (* A can depend on R *)
+  (* can r1 depend on a1 while a1 depnds on r1? *)
+  (* focus on wr0s *)
+  (* *)
+
+  (* CWX0: conditions contextuelles simples: *)
+
+  (* Simplification - read1s *)
+
+  (* Precondition: no cycles *)
+  Fixpoint get_exp_depth (e: uact) : option nat :=
+    let vars := get_vars_in_simpl_uact e in
+    let subdepths :=
+      List.map
+        (fun u => )
+        vars
+    in
+    let max :=
+      List.fold_left
+
+  Definition get_var_depth (v: string) (vvm: var_value_map) : option nat :=
+    match list_assoc vvm v with
+    | None => None
+    | Some e => Some (get_exp_depth e)
+    end.
+
+  Definition interp_cycle
+    (r: UREnv) (sigma: ext_funs_defs) (n: @normal_form pos_t reg_t ext_fn_t)
+  : UREnv :=
+    let interp_reads :=
+      List.map (fun '(reg, name) => (name, getenv REnv r reg)) (reads n)
+    in
+    (* We use the fact that the variables are recursively defined *)
+    let interp_vars :=
+      List.map (fun '(name, e) => (name, )) (reads n)
+    in
+    (* let interp_extcalls := *)
+    (* in *)
+    r.
+
+  Lemma normal_form_ok:
+    forall
+      (r: UREnv) (sigma: ext_funs_defs) (rules: rule_name_t -> uact)
+      (s: schedule) (p: pos_t)
+      (TA:
+        forall rule, exists tcr,
+        TypeInference.tc_rule TR Sigma p (rules rule) = Success tcr
+      ),
+    UntypedSemantics.interp_cycle rules r sigma s =
+    NormalForm.interp_cycle r sigma (Normalize.schedule_to_normal_form rules s).
+  Proof.
+  Admitted.
+End NormalForm.
