coq/NormalFormTactics.v
@@ -1,0 +1,6 @@
+(* Require Import Koika.Normalize. *)
+
+(* Definition *) 
+
+(* Lemma write_cond_false_implies_no_write : *)
+(* Lemma write_cond_true_implies_write_val : *)
