examples/rv/rv32i.v
@@ -76,28 +76,36 @@ Definition is_module_call
     |> Dmem |> Tick |> EndExecution |> done.
   Definition rules_desug := (fun x => (desugar_action tt (rv_urules x))).
 
-  (* Definition rules_l := schedule_to_list_of_rules rules_desug sch. *)
-  (* Definition last_action_init := *)
-  (*   list_max (List.map (get_highest_binding_id action) rules_l). *)
-  (* Definition last_expr_init := *)
-  (*   list_max (List.map (get_highest_binding_id expr) rules_l). *)
-  (* Definition resf := *)
-  (*   List.fold_left *)
-  (*     (fun '(ri_acc, la', le') r => *)
-  (*       let '(ri, la'', le'') := distill r la' le' in *)
-  (*       (ri_acc++[ri], la'', le'') *)
-  (*     ) *)
-  (*     rules_l *)
-  (*     ([], last_action_init, last_expr_init). *)
-  (* Definition rule_info_l := fst (fst resf). *)
-  (* Definition la' := snd (fst resf). *)
-  (* Definition le' := snd resf. *)
-  (* Definition rule_info_with_conflicts_l := detect_all_conflicts rule_info_l. *)
-  (* Definition schedule_info := merge_schedule rule_info_with_conflicts_l le'. *)
-  (* Definition schedule_info_simpl := *)
-  (*   remove_write0s (remove_read1s schedule_info la'). *)
+  Definition sch2 : scheduler :=
+    UpdateOnOff |> EndExecution |> Done.
 
-  Time Compute (schedule_to_normal_form rules_desug sch).
+(*   Definition rules_l := schedule_to_list_of_rules rules_desug sch2. *)
+(*   Definition last_action_init := *)
+(*     list_max (List.map (get_highest_binding_id action) rules_l). *)
+(*   Definition last_expr_init := *)
+(*     list_max (List.map (get_highest_binding_id expr) rules_l). *)
+(*   Definition resf := *)
+(*     List.fold_left *)
+(*       (fun '(ri_acc, la', le') r => *)
+(*         let '(ri, la'', le'') := distill r la' le' in *)
+(*         (ri_acc++[ri], la'', le'') *)
+(*       ) *)
+(*       rules_l *)
+(*       ([], last_action_init, last_expr_init). *)
+(*   Compute resf. *)
+(*   Definition rule_info_l := fst (fst resf). *)
+(*   Definition la' := snd (fst resf). *)
+(*   Definition le' := snd resf. *)
+(*   Definition rule_info_with_conflicts_l := detect_all_conflicts rule_info_l. *)
+(*   Definition schedule_info := merge_schedule rule_info_with_conflicts_l le'. *)
+(*   Definition schedule_info_simpl := *)
+(*     remove_write0s (remove_read1s schedule_info la'). *)
+(*   Compute rule_info_l. *)
+(*   Compute rule_info_with_conflicts_l. *)
+(*   Compute schedule_info. *)
+(*   Compute schedule_info_simpl. *)
+
+  (* Time Compute (schedule_to_normal_form rules_desug sch). *)
 
   Definition rv_rules (rl: rv_rules_t) : rule R Sigma :=
     match rl with
